Define (general) overapproximation for RPC

ExistentialRules/ChaseSequence/Nontermination/HeadChoice.lean
@@ -21,15 +21,26 @@ abbrev HeadChoice (sig : Signature) [DecidableEq sig.P] [DecidableEq sig.C] [Dec
 
 variable {sig : Signature} [DecidableEq sig.P] [DecidableEq sig.C] [DecidableEq sig.V]
 
+/-- Often we want to assume that a `HeadChoice` for equivalent triggers returns the same index. -/
+@[expose]
+def HeadChoice.consistent_for_equivalent_triggers (hc : HeadChoice sig) : Prop := ∀ {trg trg2 : PreTrigger sig}, trg.equiv trg2 -> (hc trg).val = (hc trg2).val
+
 /-- A shortcut for the trigger output dictaded by a head choice. -/
+@[expose]
 def PreTrigger.output_for_headChoice (trg : PreTrigger sig) (hc : HeadChoice sig) : List (Fact sig) :=
   trg.mapped_head[(hc trg).val]
+
+/-- The head choice output for equivalent triggers is the same given that the head choice is `consistent_for_equivalent_triggers`. -/
+theorem PreTrigger.output_for_headChoice_eq_of_equiv {trg trg2 : PreTrigger sig} {hc : HeadChoice sig}
+    (hc_consistent : hc.consistent_for_equivalent_triggers) (equiv : trg.equiv trg2) : trg.output_for_headChoice hc = trg2.output_for_headChoice hc := by
+  unfold output_for_headChoice; simp only [hc_consistent equiv, PreTrigger.result_eq_of_equiv equiv]
 
 namespace ChaseNode
 
 variable {obs : ObsolescenceCondition sig} {rules : RuleSet sig} {N : Type u} [CN : ChaseNode N obs rules]
 
 /-- A `ChaseNode` adheres to a `HeadChoice` if its origin uses the index that is the head choice of its trigger. -/
+@[expose]
 def adheres_to_headChoice (node : N) (hc : HeadChoice sig) : Prop :=
   ∀ orig ∈ (CN.origin node), orig.snd.val = (hc orig.fst.val).val
 
@@ -54,7 +65,7 @@ variable {obs : ObsolescenceCondition sig} {rules : RuleSet sig} {N : Type u} [C
 /-- The generator function used to generate the tree branch corresponding to the given `HeadChoice`. -/
 def generator_for_headChoice (td : TreeDerivation N obs rules) (hc : HeadChoice sig) (n : td.NodeWithAddress) : Option td.NodeWithAddress :=
   let next_trg_opt : Option (PreTrigger sig) := (n.childNodes.head?.bind (fun c => CN.origin c.node)).map (fun o => o.fst.val)
-  next_trg_opt.bind (fun trg => n.childNodes[hc trg]?)
+  next_trg_opt.bind (fun trg => n.childNodes[(hc trg).val]?)
 
 /-- The generator function produces a child node if it produces a value at all. -/
 theorem generator_for_headChoice_mem_childNodes {td : TreeDerivation N obs rules} {hc : HeadChoice sig} (n : td.NodeWithAddress) :
@@ -89,6 +100,27 @@ theorem generator_for_headChoice_eq_none_iff_childNodes_eq_nil {td : TreeDerivat
       apply Nat.not_le_of_lt this; rw [n.childNodes_eq_childNodes]; simp only [List.length_map]; rw [← List.getElem?_eq_none_iff]; exact contra
     rw [ingoing_eq, List.length_map, PreTrigger.length_mapped_head]; exact (hc trg.val).isLt
 
+/-- The node produced by `generator_for_headChoice` adheres to the head choice. -/
+theorem generator_for_headChoice_adheres_to_headChoice {td : TreeDerivation N obs rules} {hc : HeadChoice sig} (n : td.NodeWithAddress) :
+    ∀ next ∈ td.generator_for_headChoice hc n, CN.adheres_to_headChoice next.node hc := by
+  intro next next_mem orig orig_mem; simp only [generator_for_headChoice, Option.mem_def, Option.bind_eq_some_iff] at next_mem
+  rcases next_mem with ⟨head_trg, head_trg_eq, next_mem⟩
+  have childNodes_ne_nil : n.childNodes ≠ [] := by apply List.ne_nil_of_mem; rw [List.mem_iff_getElem?]; exact ⟨_, next_mem⟩
+  rcases n.triggers_exist (by rw [TreeDerivation.NodeWithAddress.childNodes_eq_childNodes]; intro contra; rw [List.map_eq_nil_iff] at contra; apply childNodes_ne_nil; exact contra) with ⟨trg, act, ingoing_eq, trg_eq, orig_eq⟩
+  specialize orig_eq (next.node, (hc head_trg).val) (by simp only [List.mem_zipIdx_iff_getElem?, TreeDerivation.NodeWithAddress.childNodes_eq_childNodes, List.getElem?_map]; rw [next_mem]; simp)
+  rw [Option.mem_def] at orig_mem
+  simp only [orig_mem, Option.map_some, Option.some_inj] at orig_eq
+  rw [orig_eq]
+  suffices head_trg = orig.fst.val by rw [this]
+  have trg_eq' := trg_eq next.node (by rw [TreeDerivation.NodeWithAddress.childNodes_eq_childNodes]; apply List.mem_map_of_mem; apply List.mem_of_getElem?; exact next_mem)
+  rw [orig_mem, Option.map_some, Option.some_inj] at trg_eq'
+  rw [trg_eq']
+  rw [List.head?_eq_some_head childNodes_ne_nil, Option.bind_some] at head_trg_eq
+  have trg_eq' := trg_eq (n.childNodes.head childNodes_ne_nil).node (by rw [TreeDerivation.NodeWithAddress.childNodes_eq_childNodes]; apply List.mem_map_of_mem; exact List.head_mem _)
+  rw [Option.map_eq_some_iff] at trg_eq'; rcases trg_eq' with ⟨head_orig, trg_eq'⟩
+  rw [trg_eq'.left, Option.map_some, Option.some_inj] at head_trg_eq
+  rw [← head_trg_eq, trg_eq'.right]
+
 /-- This function generates the tree branch that corresponds to the given `HeadChoice`. -/
 def subderivation_for_headChoice (td : TreeDerivation N obs rules) (hc : HeadChoice sig) : ChaseDerivation N obs rules :=
   td.generate_subderivation (NodeWithAddress.root td) (td.generator_for_headChoice hc) id td.generator_for_headChoice_mem_childNodes (by intro n; rw [generator_for_headChoice_eq_none_iff_childNodes_eq_nil]; rw [List.eq_nil_iff_length_eq_zero, List.eq_nil_iff_length_eq_zero, n.length_childNodes, n.subderivation.childNodes_eq]; simp)
@@ -100,6 +132,22 @@ theorem subderivation_for_headChoice_mem_branches {td : TreeDerivation N obs rul
 /-- The head of `subderivation_for_headChoice` is the root of the tree derivation. -/
 theorem head_subderivation_for_headChoice {td : TreeDerivation N obs rules} {hc : HeadChoice sig} :
   (td.subderivation_for_headChoice hc).head = td.root := td.head_generate_subderivation
+
+/-- The subderivation for a head choice adheres to that head choice. -/
+theorem subderivation_for_headChoice_adheres_to_headChoice_of_root_adheres {td : TreeDerivation N obs rules} {hc : HeadChoice sig} :
+    CN.adheres_to_headChoice td.root hc -> (td.subderivation_for_headChoice hc).adheres_to_headChoice hc := by
+  simp only [subderivation_for_headChoice]
+  intro root_adheres node node_mem; rw [← ChaseDerivation.mem_def, td.mem_generate_subderivation] at node_mem
+  rcases node_mem with ⟨n, node_mem⟩
+  cases n with
+  | zero => simp only [Function.repeat_zero, Option.map_some, Option.mem_some] at node_mem; rw [← node_mem]; exact root_adheres
+  | succ n =>
+    rw [Function.repeat_succ, Option.mem_def, Option.map_map, Option.map_eq_some_iff] at node_mem
+    rcases node_mem with ⟨next, next_mem, node_mem⟩
+    rw [Option.bind_eq_some_iff] at next_mem; rcases next_mem with ⟨_, _, goal⟩
+    rw [← node_mem]
+    apply generator_for_headChoice_adheres_to_headChoice
+    exact goal
 
 end TreeDerivation
 
@@ -119,6 +167,12 @@ def subderivation_for_headChoice (ct : ChaseTree N obs kb) (hc : HeadChoice sig)
     fairness := deriv.fairness,
     database_first := by rw [TreeDerivation.head_subderivation_for_headChoice]; exact ct.database_first
   }
+
+/-- The subderivation for a head choice adheres to that head choice. -/
+theorem subderivation_for_headChoice_adheres_to_headChoice {ct : ChaseTree N obs kb} {hc : HeadChoice sig} :
+    (ct.subderivation_for_headChoice hc).adheres_to_headChoice hc := by
+  apply TreeDerivation.subderivation_for_headChoice_adheres_to_headChoice_of_root_adheres
+  intro orig orig_mem; rw [ct.database_first.right.right] at orig_mem; simp at orig_mem
 
 end ChaseTree
 
